monpred: Add `BiIndex{,Element}Discrete`

theories/lang/bi/monpred.v
@@ -29,3 +29,50 @@ Section proofmode_monpred.
     MakeMonPredAt i [|φ|] [|φ|].
   Proof. rewrite /MakeMonPredAt. by rewrite monPred_at_only_provable. Qed.
 End proofmode_monpred.
+
+(** ** Discrete BI indices and discrete BI index elements *)
+(**
+We might eventually need to generalize from Leibniz equality to setoid
+equivalence. Should that happen, we might want to (in stdpp),
+generalize so as to use the same typeclasses for these things and
+Iris' [Discrete], [OfeDiscrete].
+*)
+
+Class BiIndexElementDiscrete {I : biIndex} (i : I) : Prop :=
+  bi_index_element_discrete i' : i ⊑ i' → i = i'.
+#[global] Hint Mode BiIndexElementDiscrete + ! : typeclass_instances.
+#[global] Hint Opaque BiIndexElementDiscrete : typeclass_instances.
+#[global] Instance: Params (@BiIndexElementDiscrete) 1 := {}.
+#[global] Instance: Params (@bi_index_element_discrete) 4 := {}.
+#[global] Arguments bi_index_element_discrete {_} _ {_} _ _ : assert.
+
+Class BiIndexDiscrete (I : biIndex) : Prop :=
+  bi_index_discrete (i : I) :> BiIndexElementDiscrete i.
+#[global] Hint Mode BiIndexDiscrete ! : typelcass_instances.
+
+Section bi_index_discrete.
+  Context {I : biIndex}.
+  Implicit Type i : I.
+
+  #[global] Instance BiIndexElementDiscrete_mono :
+    Proper ((⊑) ==> impl) (@BiIndexElementDiscrete I).
+  Proof.
+    intros i1 i2 Hi ? i' Hi'.
+    generalize (bi_index_element_discrete _ _ Hi). intros ->.
+    by apply bi_index_element_discrete.
+  Qed.
+  #[global] Instance BiIndexElementDiscrete_flip_mono :
+    Proper (flip (⊑) ==> flip impl) (@BiIndexElementDiscrete I).
+  Proof. repeat intro. exact: BiIndexElementDiscrete_mono. Qed.
+
+  Lemma bi_index_element_discrete_iff i `{!BiIndexElementDiscrete i} i' :
+    i ⊑ i' ↔ i = i'.
+  Proof. split. by apply bi_index_element_discrete. by move=>->. Qed.
+
+  (**
+  Setting aside typeclass resolution hints, these two are equivalent.
+  *)
+  Lemma subrelation_bi_index_discrete :
+    @subrelation I (⊑) (=) ↔ BiIndexDiscrete I.
+  Proof. done. Qed.
+End bi_index_discrete.
